lib/zoo_std/queue_2.ml
@@ -2,35 +2,35 @@ type ('a, _) node =
   | Null :
     ('a, [> `Null]) node
   | Node :
-    { mutable head: 'a;
-      mutable tail: ('a, [`Null | `Node]) node;
+    { mutable next: ('a, [`Null | `Node]) node;
+      mutable data: 'a;
     } ->
     ('a, [> `Node]) node
 
 type 'a t =
   { mutable front: ('a, [`Node]) node;
-    mutable sentinel: ('a, [`Node]) node;
+    mutable back: ('a, [`Node]) node;
   }
 
 let create () =
-  let sent = Node { head= Obj.magic (); tail= Null } in
-  { front= sent; sentinel= sent }
+  let front = Node { next= Null; data= Obj.magic () } in
+  { front; back= front }
 
 let is_empty t =
-  t.front == t.sentinel
+  t.front == t.back
 
 let push t v =
-  let (Node _ as new_sent : (_, [`Node]) node) = Node { head= Obj.magic (); tail= Null } in
-  let Node sent_r = t.sentinel in
-  sent_r.head <- v ;
-  sent_r.tail <- new_sent ;
-  t.sentinel <- new_sent
+  let (Node _ as new_back : (_, [`Node]) node) = Node { next= Null; data= Obj.magic () } in
+  let Node back_r = t.back in
+  back_r.next <- new_back ;
+  back_r.data <- v ;
+  t.back <- new_back
 
 let pop t =
   let Node front_r = t.front in
-  match front_r.tail with
+  match front_r.next with
   | Null ->
       None
-  | Node _ as tail ->
-      t.front <- tail ;
-      Some front_r.head
+  | Node _ as next ->
+      t.front <- next ;
+      Some front_r.data
