theories/zoo_std/queue_2.v
@@ -1,14 +1,161 @@
 From zoo Require Import
   prelude.
+From zoo.language Require Import
+  notations.
+From zoo.diaframe Require Import
+  diaframe.
 From zoo_std Require Export
   base
   queue_2__code.
 From zoo_std Require Import
+  option
+  chain
   queue_2__types.
 From zoo Require Import
   options.
+
+Implicit Types l : location.
+Implicit Types t v front back : val.
+Implicit Types vs : list val.
+
+Section zoo_G.
+  Context `{zoo_G : !ZooG Σ}.
+
+  Definition queue_2_model t vs : iProp Σ :=
+    ∃ l front back,
+    ⌜t = #l⌝ ∗
+    l.[front] ↦ front ∗
+    l.[back] ↦ back ∗
+    chain_model (Some §Node) front vs back ∗
+    chain_model (Some §Node) back [()%V] ().
+  #[local] Instance : CustomIpatFormat "model" :=
+    "(
+      %l &
+      %front &
+      %back &
+      -> &
+      Hl_front &
+      Hl_back &
+      Hfront &
+      Hback
+    )".
+
+  #[global] Instance queue_2_model_timeless t vs :
+    Timeless (queue_2_model t vs).
+  Proof.
+    apply _.
+  Qed.
+
+  Lemma queue_2_create_spec :
+    {{{
+      True
+    }}}
+      queue_2_create ()
+    {{{ t,
+      RET t;
+      queue_2_model t []
+    }}}.
+  Proof.
+    iIntros "%Φ _ HΦ".
+    wp_rec.
+    wp_apply (chain_block_spec (Some _)) as (back) "Hback_model".
+    { iApply chain_model_nil. iSteps. }
+    wp_block l as "(Hfront & Hback & _)".
+    iApply "HΦ". iExists l, back, back. iFrame. iSteps.
+    iApply chain_model_nil. iSteps.
+  Qed.
+
+  Lemma queue_2_is_empty_spec t vs :
+    {{{
+      queue_2_model t vs
+    }}}
+      queue_2_is_empty t
+    {{{
+      RET #(bool_decide (vs = []%list));
+      queue_2_model t vs
+    }}}.
+  Proof.
+    iIntros "%Φ (:model) HΦ".
+    wp_rec. do 2 wp_load.
+    destruct vs as [| v vs].
+    - iDestruct (chain_model_nil with "Hfront") as %->.
+      iDestruct (chain_physical with "Hback") as %Hphysical; first naive_solver.
+      wp_equal as ? | _.
+      { iDestruct (chain_physically_distinct' with "Hback") as %[]; naive_solver. }
+      iSteps.
+    - wp_apply (wp_equal_chain with "Hfront Hback") as "Hfront Hback"; [naive_solver lia.. |].
+      iSplit; first iSteps. iIntros "->".
+      iDestruct (chain_model_exclusive with "Hback Hfront") as %[]; naive_solver lia.
+  Qed.
+
+  Lemma queue_2_push_spec t vs v :
+    {{{
+      queue_2_model t vs
+    }}}
+      queue_2_push t v
+    {{{
+      RET ();
+      queue_2_model t (vs ++ [v])
+    }}}.
+  Proof.
+    iIntros "%Φ (:model) HΦ".
+    wp_rec.
+    wp_smart_apply (chain_block_spec (Some _)) as (back') "Hback'".
+    { iApply chain_model_nil. iSteps. }
+    iDestruct (chain_model_tag with "Hback'") as "#(%back'_ & -> & Hback'_hdr)"; first done. wp_match.
+    wp_load.
+    iDestruct (chain_model_tag with "Hback") as "#(%back_ & -> & Hback_hdr)"; first done. wp_match.
+    wp_smart_apply (chain_set_next_spec with "Hback") as (?) "(Hback & _)".
+    wp_smart_apply (chain_set_data_spec with "Hback") as "Hback".
+    iDestruct (chain_model_app_2 with "Hfront Hback") as "Hfront".
+    iSteps.
+  Qed.
+
+  Lemma queue_2_pop_spec t vs :
+    {{{
+      queue_2_model t vs
+    }}}
+      queue_2_pop t
+    {{{
+      RET (head vs : val);
+      queue_2_model t (tail vs)
+    }}}.
+  Proof.
+    iIntros "%Φ (:model) HΦ".
+    wp_rec. wp_load.
+
+    iAssert (
+      ∃ front_ : location,
+      ⌜front = #front_⌝ ∗
+      front_ ↦ₕ Header §Node 2
+    )%I as "(%front_ & -> & #Hfront_hdr)".
+    { iDestruct (chain_model_app_2 with "Hfront Hback") as "Hfront".
+      iApply (chain_model_tag with "Hfront").
+      { rewrite length_app /=. lia. }
+    }
+
+    wp_match.
+    destruct vs as [| v1 vs].
+    - iDestruct (chain_model_nil with "Hfront") as %->.
+      wp_apply (chain_next_spec_singleton with "Hback") as "Hback".
+      iSteps.
+    - wp_apply (chain_next_spec with "Hfront") as (front') "(Hfront & Hfront')".
+      destruct vs as [| v2 vs].
+      + iDestruct (chain_model_nil with "Hfront'") as %->.
+        iDestruct (chain_model_tag with "Hback") as "#(%back_ & -> & Hback_hdr)"; first done. wp_match.
+        wp_store.
+        wp_smart_apply (chain_data_spec with "Hfront") as "Hfront".
+        iSteps.
+      + iDestruct (chain_model_tag with "Hfront'") as "#(%front'_ & -> & Hfront'_hdr)"; first done. wp_match.
+        wp_store.
+        wp_smart_apply (chain_data_spec with "Hfront") as "Hfront".
+        iSteps.
+  Qed.
+End zoo_G.
 
 #[global] Opaque queue_2_create.
 #[global] Opaque queue_2_is_empty.
 #[global] Opaque queue_2_push.
 #[global] Opaque queue_2_pop.
+
+#[global] Opaque queue_2_model.
