theories/zoo_std/queue_1__types.v
@@ -12,7 +12,7 @@ Notation "'front'" := (
   in_type "t" 0
 )(in custom zoo_field
 ).
-Notation "'sentinel'" := (
+Notation "'back'" := (
   in_type "t" 1
 )(in custom zoo_field
 ).
